add Vec

Lambda/Fin.lean
@@ -5,3 +5,18 @@ inductive Fin' : Nat → Type where
 def Fin'.ofNat : ∀ {m} (n), n < m → Fin' m
 | _ + 1, 0, _ => fz
 | _ + 1, (n + 1), h => fs (Fin'.ofNat n (Nat.le_of_succ_le_succ h))
+
+inductive Vec (α : Type u) : Nat → Type u where
+| nil : Vec α 0
+| cons : α → Vec α n → Vec α (n + 1)
+
+notation "[]ᵥ" => Vec.nil
+infixr:55 " ∷ᵥ " => Vec.cons
+
+instance : EmptyCollection (Vec α 0) := ⟨[]ᵥ⟩
+@[simp] def Vec.add (v : Vec α n) (x : α) := x ∷ᵥ v
+infixl:55 ",' " => Vec.add
+
+def Vec.get : Vec α n → Fin' n → α
+| a ∷ᵥ _, Fin'.fz => a
+| _ ∷ᵥ v, Fin'.fs x => v.get x
